Manually construct tvsubst for POPLmark 2B

thys/POPLmark/POPLmark_2B.thy
@@ -2,12 +2,923 @@ theory POPLmark_2B
 imports POPLmark_1B
 begin
 
-binder_datatype (FTVars: 'tv, FVars: 'v) trm = Var 'v
+binder_datatype (FTVars: 'tv, FVars: 'v) trm =
+    Var 'v
   | Abs x::'v "'tv typ" t::"('tv, 'v) trm" binds x in t
   | App "('tv, 'v) trm" "('tv, 'v) trm"
   | TAbs X::'tv "'tv typ" t::"('tv, 'v) trm" binds X in t
   | TApp "('tv, 'v) trm" "'tv typ"
 print_theorems
+
+definition tvsubst_trm_pre :: "('tv::var \<Rightarrow> 'tv typ) \<Rightarrow> ('tv, 'v::var, 'tv, 'v, 'a, 'b) trm_pre \<Rightarrow> ('tv, 'v, 'tv, 'v, 'a, 'b) trm_pre" where
+  "tvsubst_trm_pre f x \<equiv> Abs_trm_pre (case Rep_trm_pre x of
+    Inl (Inr (x, T, t)) \<Rightarrow> Inl (Inr (x, tvsubst_typ f T, t))
+  | Inr (Inr (Inl (x, T, t))) \<Rightarrow> Inr (Inr (Inl (x, tvsubst_typ f T, t)))
+  | Inr (Inr (Inr (t, T))) \<Rightarrow> Inr (Inr (Inr (t, tvsubst_typ f T)))
+  | x \<Rightarrow> x
+  )"
+abbreviation \<eta> :: "'v \<Rightarrow> ('tv::var, 'v::var, 'btv::var, 'bv::var, 'a, 'b) trm_pre" where
+  "\<eta> a \<equiv> Abs_trm_pre (Inl (Inl a))"
+
+lemma eta_free: "set2_trm_pre (\<eta> a) = {a}"
+  apply (unfold set2_trm_pre_def sum.set_map UN_empty2 Un_empty_left Un_empty_right prod.set_map comp_def
+    Abs_trm_pre_inverse[OF UNIV_I] sum_set_simps UN_empty UN_single
+  )
+  apply (rule refl)
+  done
+lemma eta_inj: "\<eta> a = \<eta> b \<Longrightarrow> a = b"
+  apply (unfold Abs_trm_pre_inject[OF UNIV_I UNIV_I] sum.inject)
+  apply assumption
+  done
+lemma eta_natural:
+  fixes f1::"'x1::var \<Rightarrow> 'x1" and f2::"'x2::var \<Rightarrow> 'x2" and f3::"'x3::var \<Rightarrow> 'x3" and f4::"'x4::var \<Rightarrow> 'x4"
+  assumes "|supp f1| <o |UNIV::'x1 set|" "|supp f2| <o |UNIV::'x2 set|"
+    "bij f3" "|supp f3| <o |UNIV::'x3 set|" "bij f4" "|supp f4| <o |UNIV::'x4 set|"
+  shows "map_trm_pre f1 f2 f3 f4 f5 f6 \<circ> \<eta> = \<eta> \<circ> f2"
+  apply (rule ext)
+  apply (unfold comp_def map_trm_pre_def Abs_trm_pre_inverse[OF UNIV_I] map_sum.simps)
+  apply (rule refl)
+  done
+
+(* Construction of substitution *)
+type_synonym ('tv, 'v) P = "('v \<Rightarrow> ('tv, 'v) trm) \<times> ('tv \<Rightarrow> 'tv typ)"
+
+definition VVr :: "'v::var \<Rightarrow> ('tv::var, 'v) trm" where
+  "VVr \<equiv> trm_ctor \<circ> \<eta>"
+definition isVVr :: "('tv::var, 'v::var) trm \<Rightarrow> bool" where
+  "isVVr x \<equiv> \<exists>a. x = VVr a"
+definition asVVr :: "('tv::var, 'v::var) trm \<Rightarrow> 'v" where
+  "asVVr x \<equiv> (if isVVr x then SOME a. x = VVr a else undefined)"
+
+definition Uctor :: "('tv::var, 'v::var, 'tv, 'v, ('tv, 'v) trm \<times> (('tv, 'v) P \<Rightarrow> ('tv, 'v) trm), ('tv, 'v) trm \<times> (('tv, 'v) P \<Rightarrow> ('tv, 'v) trm)) trm_pre
+  \<Rightarrow> ('tv, 'v) P \<Rightarrow> ('tv, 'v) trm" where
+  "Uctor y p \<equiv> case p of (f1, f2) \<Rightarrow> if isVVr (trm_ctor (map_trm_pre id id id id fst fst y)) then
+    f1 (asVVr (trm_ctor (map_trm_pre id id id id fst fst y)))
+  else
+    trm_ctor (tvsubst_trm_pre f2 (map_trm_pre id id id id ((\<lambda>R. R (f1, f2)) \<circ> snd) ((\<lambda>R. R (f1, f2)) \<circ> snd) y))"
+
+definition PFVars_1 :: "('tv::var, 'v::var) P \<Rightarrow> 'tv set" where
+  "PFVars_1 p \<equiv> case p of (f1, f2) \<Rightarrow> IImsupp_1_trm f1 \<union> IImsupp_typ f2"
+definition PFVars_2 :: "('tv::var, 'v::var) P \<Rightarrow> 'v set" where
+  "PFVars_2 p \<equiv> case p of (f1, _) \<Rightarrow> IImsupp_2_trm f1"
+
+definition compSS_typ :: "('tv \<Rightarrow> 'tv) \<Rightarrow> ('tv \<Rightarrow> 'tv::var typ) \<Rightarrow> 'tv \<Rightarrow> 'tv typ" where
+  "compSS_typ g f \<equiv> permute_typ g \<circ> f \<circ> inv g"
+definition compSS_trm :: "('tv \<Rightarrow> 'tv) \<Rightarrow> ('v \<Rightarrow> 'v) \<Rightarrow> ('v \<Rightarrow> ('tv::var, 'v::var) trm) \<Rightarrow> 'v \<Rightarrow> ('tv, 'v) trm" where
+  "compSS_trm g1 g2 f \<equiv> permute_trm g1 g2 \<circ> f \<circ> inv g2"
+definition Pmap :: "('tv \<Rightarrow> 'tv) \<Rightarrow> ('v \<Rightarrow> 'v) \<Rightarrow> ('tv::var, 'v::var) P \<Rightarrow> ('tv, 'v) P" where
+  "Pmap g1 g2 p \<equiv> case p of (f1, f2) \<Rightarrow> (compSS_trm g1 g2 f1, compSS_typ g1 f2)"
+lemmas compSS_defs = compSS_typ_def compSS_trm_def
+
+definition valid_P :: "('tv::var, 'v::var) P \<Rightarrow> bool" where
+  "valid_P p \<equiv> case p of (f1, f2) \<Rightarrow>
+    |SSupp_trm f1| <o cmin |UNIV::'tv set| |UNIV::'v set|
+  \<and> |SSupp_typ f2| <o cmin |UNIV::'tv set| |UNIV::'v set|"
+
+lemma asVVr_VVr: "asVVr (VVr a) = a"
+  apply (unfold asVVr_def isVVr_def)
+  apply (subst if_P)
+   apply (rule exI)
+   apply (rule refl)
+  apply (rule someI2)
+   apply (rule refl)
+  apply (unfold VVr_def comp_def)
+  apply (unfold trm.TT_inject0)
+  apply (erule exE conjE)+
+  apply (unfold map_trm_pre_def comp_def Abs_trm_pre_inverse[OF UNIV_I]
+    map_sum.simps Abs_trm_pre_inject[OF UNIV_I UNIV_I] id_apply
+    sum.inject
+  )
+  apply (erule sym)
+  done
+
+lemma permute_VVr:
+  fixes f1::"'var::var \<Rightarrow> 'var" and f2::"'tyvar::var \<Rightarrow> 'tyvar"
+  assumes f_prems: "bij f1" "|supp f1| <o |UNIV::'var set|" "bij f2" "|supp f2| <o |UNIV::'tyvar set|"
+  shows "permute_trm f1 f2 (VVr a) = VVr (f2 a)"
+  apply (unfold VVr_def comp_def)
+  apply (rule trans)
+   apply (rule trm.permute_ctor[OF assms])
+  apply (subst fun_cong[OF eta_natural, unfolded comp_def])
+      apply (rule assms)+
+  apply (rule refl)
+  done
+
+lemma isVVr_permute:
+  fixes f1::"'var::var \<Rightarrow> 'var" and f2::"'tyvar::var \<Rightarrow> 'tyvar"
+  assumes f_prems: "bij f1" "|supp f1| <o |UNIV::'var set|" "bij f2" "|supp f2| <o |UNIV::'tyvar set|"
+  shows "isVVr (permute_trm f1 f2 x) = isVVr x"
+  apply (unfold isVVr_def)
+  apply (rule iffI)
+   apply (erule exE)
+   apply (drule arg_cong[of _ _ "permute_trm (inv f1) (inv f2)"])
+   apply (subst (asm) trm.permute_comp)
+           apply (rule assms bij_imp_bij_inv supp_inv_bound)+
+   apply (subst (asm) inv_o_simp1, rule assms)+
+   apply (unfold trm.permute_id)
+   apply hypsubst_thin
+   apply (subst permute_VVr)
+       apply (rule assms bij_imp_bij_inv supp_inv_bound)+
+   apply (rule exI)
+   apply (rule refl)
+  apply (erule exE)
+  apply hypsubst_thin
+  apply (subst permute_VVr)
+      apply (rule assms bij_imp_bij_inv supp_inv_bound)+
+  apply (rule exI)
+  apply (rule refl)
+  done
+
+lemma compSS_id0s:
+  "compSS_typ id = id"
+  "compSS_trm id id = id"
+  apply (unfold compSS_typ_def compSS_trm_def trm.permute_id0 typ.permute_id0 id_o o_id inv_id)
+  apply (unfold id_def)
+  apply (rule refl)+
+  done
+
+lemma compSS_comp0_trm:
+  fixes f1 g1::"'tyvar::var \<Rightarrow> 'tyvar" and f2 g2::"'var::var \<Rightarrow> 'var"
+  assumes g_prems: "bij g1" "|supp g1| <o cmin |UNIV::'tyvar set| |UNIV::'var set|" "bij g2" "|supp g2| <o cmin |UNIV::'tyvar set| |UNIV::'var set|"
+    and f_prems: "bij f1" "|supp f1| <o cmin |UNIV::'tyvar set| |UNIV::'var set|" "bij f2" "|supp f2| <o cmin |UNIV::'tyvar set| |UNIV::'var set|"
+  shows
+    "compSS_trm f1 f2 \<circ> compSS_trm g1 g2 = compSS_trm (f1 \<circ> g1) (f2 \<circ> g2)"
+  apply (unfold compSS_trm_def)
+  apply (subst o_inv_distrib trm.permute_comp0[symmetric], (rule supp_id_bound bij_id assms ordLess_ordLeq_trans cmin2 cmin1 card_of_Card_order)+)+
+  apply (rule ext)
+  apply (rule trans[OF comp_apply])
+  apply (unfold comp_assoc)
+  apply (rule refl)
+  done
+lemmas compSS_comp0s = typ.compSS_comp0[unfolded tvcompSS_tvsubst_typ_def compSS_typ_def[symmetric]] compSS_comp0_trm
+
+lemma IImsupp_VVrs: "f2 a \<noteq> a \<Longrightarrow> imsupp f2 \<inter> IImsupp_2_trm y = {} \<Longrightarrow> y a = VVr a"
+  apply (unfold imsupp_def supp_def IImsupp_2_trm_def SSupp_trm_def tvVVr_tvsubst_trm_def tv\<eta>_trm_tvsubst_trm_def VVr_def[symmetric])
+  apply (drule iffD1[OF disjoint_iff])
+  apply (erule allE)
+  apply (erule impE)
+   apply (rule UnI1)
+   apply (erule iffD2[OF mem_Collect_eq])
+  apply (unfold Un_iff de_Morgan_disj mem_Collect_eq not_not)
+  apply (erule conjE)
+  apply assumption
+  done
+
+lemma IImsupp_permute_commute:
+  fixes f1::"'var::var \<Rightarrow> 'var" and f2::"'tyvar::var \<Rightarrow> 'tyvar"
+  assumes f_prems: "bij f1" "|supp f1| <o |UNIV::'var set|" "bij f2" "|supp f2| <o |UNIV::'tyvar set|"
+  shows "imsupp f1 \<inter> IImsupp_1_trm y = {} \<Longrightarrow> imsupp f2 \<inter> IImsupp_2_trm y = {} \<Longrightarrow> permute_trm f1 f2 \<circ> y = y \<circ> f2"
+  apply (rule ext)
+  apply (unfold comp_def)
+  subgoal for a
+    apply (rule case_split[of "f2 a = a"])
+     apply (rule case_split[of "y a = VVr a"])
+      apply (rule trans)
+       apply (rule arg_cong[of _ _ "permute_trm f1 f2"])
+       apply assumption
+      apply (rule trans)
+       apply (rule permute_VVr)
+          apply (rule assms)+
+      apply (rule trans)
+       apply (rule arg_cong[of _ _ VVr])
+       apply assumption
+      apply (rule sym)
+      apply (rotate_tac -2)
+      apply (erule subst[OF sym])
+      apply assumption
+
+     apply (rule trans)
+      apply (rule trm.permute_cong_id)
+           apply (rule assms)+
+      (* REPEAT_DETERM *)
+       apply (erule id_onD[rotated])
+       apply (rule imsupp_id_on)
+       apply (erule Int_subset_empty2)
+       apply (unfold IImsupp_1_trm_def SSupp_trm_def tvVVr_tvsubst_trm_def tv\<eta>_trm_tvsubst_trm_def VVr_def[symmetric])[1]
+       apply (unfold comp_def)[1]
+       apply (rule subsetI)
+       apply (rule UnI2)?
+       apply (rule UN_I[rotated])
+        apply assumption
+       apply (rule CollectI)
+       apply assumption
+      (* repeated *)
+      (* REPEAT_DETERM *)
+      apply (erule id_onD[rotated])
+      apply (rule imsupp_id_on)
+      apply (erule Int_subset_empty2)
+      apply (unfold IImsupp_2_trm_def SSupp_trm_def tvVVr_tvsubst_trm_def tv\<eta>_trm_tvsubst_trm_def VVr_def[symmetric])[1]
+       apply (unfold comp_def)[1]
+      apply (rule subsetI)
+      apply (rule UnI2)?
+      apply (rule UN_I[rotated])
+       apply assumption
+      apply (rule CollectI)
+      apply assumption
+      (* END REPEAT_DETERM *)
+     apply (rotate_tac -2)
+     apply (erule subst[OF sym])
+     apply (rule refl)
+
+    apply (rule trans)
+     apply (rule arg_cong[of _ _ "permute_trm f1 f2"])
+     defer
+     apply (rule trans)
+      prefer 3
+      apply (erule IImsupp_VVrs)
+      apply assumption
+     apply (rule permute_VVr)
+        apply (rule f_prems)+
+    apply (rule sym)
+    apply (rule IImsupp_VVrs)
+     apply (erule bij_not_eq_twice[rotated])
+     apply (rule f_prems)
+    apply assumption
+    done
+  done
+
+lemma compSS_cong_id_trm:
+  fixes f1 g1::"'tyvar::var \<Rightarrow> 'tyvar" and f2 g2::"'var::var \<Rightarrow> 'var"
+  assumes g_prems: "bij g1" "|supp g1| <o cmin |UNIV::'tyvar set| |UNIV::'var set|" "bij g2" "|supp g2| <o cmin |UNIV::'tyvar set| |UNIV::'var set|"
+    and f_prems: "bij f1" "|supp f1| <o cmin |UNIV::'tyvar set| |UNIV::'var set|" "bij f2" "|supp f2| <o cmin |UNIV::'tyvar set| |UNIV::'var set|"
+  shows
+    "(\<And>a. a \<in> IImsupp_1_trm h \<Longrightarrow> f1 a = a) \<Longrightarrow> (\<And>a. a \<in> IImsupp_2_trm h \<Longrightarrow> f2 a = a) \<Longrightarrow> compSS_trm f1 f2 h = h"
+  apply (unfold compSS_trm_def)
+  subgoal premises prems
+    apply (subst IImsupp_permute_commute)
+          apply (rule assms cmin1 cmin2 card_of_Card_order ordLess_ordLeq_trans)+
+    (* REPEAT_DETERM *)
+      apply (rule trans[OF Int_commute])
+      apply (rule disjointI)
+      apply (drule prems)
+      apply (erule bij_id_imsupp[rotated])
+      apply (rule assms)
+    (* repeated *)
+      apply (rule trans[OF Int_commute])
+      apply (rule disjointI)
+      apply (drule prems)
+      apply (erule bij_id_imsupp[rotated])
+      apply (rule assms)
+    (* END REPEAT_DETERM *)
+    apply (unfold comp_assoc)
+    apply (subst inv_o_simp2)
+     apply (rule assms)
+    apply (rule o_id)
+    done
+  done
+
+lemmas compSS_cong_ids = typ.compSS_cong_id[unfolded tvcompSS_tvsubst_typ_def compSS_typ_def[symmetric]] compSS_cong_id_trm
+lemmas SSupp_naturals = typ.SSupp_natural trm.SSupp_natural
+lemmas IImsupp_naturals = typ.IImsupp_natural trm.IImsupp_natural
+
+(* Recursor axioms *)
+lemma Pmap_id0: "Pmap id id = id"
+  apply (rule ext)
+  apply (unfold Pmap_def case_prod_beta compSS_id0s)
+  apply (unfold id_def prod.collapse)
+  apply (rule refl)
+  done
+
+lemma Pmap_comp0:
+  fixes f1 g1::"'tyvar::var \<Rightarrow> 'tyvar" and f2 g2::"'var::var \<Rightarrow> 'var"
+  assumes g_prems: "bij g1" "|supp g1| <o cmin |UNIV::'tyvar set| |UNIV::'var set|" "bij g2" "|supp g2| <o cmin |UNIV::'tyvar set| |UNIV::'var set|"
+    and f_prems: "bij f1" "|supp f1| <o cmin |UNIV::'tyvar set| |UNIV::'var set|" "bij f2" "|supp f2| <o cmin |UNIV::'tyvar set| |UNIV::'var set|"
+  shows
+    "Pmap f1 f2 \<circ> Pmap g1 g2 = Pmap (f1 \<circ> g1) (f2 \<circ> g2)"
+  apply (rule ext)
+  apply (unfold Pmap_def case_prod_beta)
+  apply (rule trans[OF comp_apply])
+  apply (unfold prod.inject fst_conv snd_conv)
+  apply (rule conjI bij_id supp_id_bound assms ordLess_ordLeq_trans cmin1 card_of_Card_order
+      trans[OF comp_apply[symmetric] fun_cong[OF compSS_comp0s(1)]]
+      trans[OF comp_apply[symmetric] fun_cong[OF compSS_comp0s(2)]]
+      )+
+  done
+
+lemma valid_Pmap:
+  fixes f1::"'tyvar::var \<Rightarrow> 'tyvar" and f2::"'var::var \<Rightarrow> 'var"
+  assumes f_prems: "bij f1" "|supp f1| <o cmin |UNIV::'tyvar set| |UNIV::'var set|" "bij f2" "|supp f2| <o cmin |UNIV::'tyvar set| |UNIV::'var set|"
+  shows "valid_P p \<Longrightarrow> valid_P (Pmap f1 f2 p)"
+  apply (unfold valid_P_def Pmap_def case_prod_beta compSS_defs fst_conv snd_conv)
+  apply (erule conj_forward)+
+   apply (subst SSupp_naturals; (assumption | rule assms cmin1 cmin2 card_of_Card_order ordLeq_ordLess_trans[OF card_of_image] ordLess_ordLeq_trans)+)+
+  done
+
+lemma PFVars_Pmaps:
+  fixes f1::"'tyvar::var \<Rightarrow> 'tyvar" and f2::"'var::var \<Rightarrow> 'var"
+  assumes f_prems: "bij f1" "|supp f1| <o cmin |UNIV::'tyvar set| |UNIV::'var set|" "bij f2" "|supp f2| <o cmin |UNIV::'tyvar set| |UNIV::'var set|"
+  shows "PFVars_1 (Pmap f1 f2 p) = f1 ` PFVars_1 p"
+    "PFVars_2 (Pmap f1 f2 p) = f2 ` PFVars_2 p"
+  subgoal
+    apply (unfold PFVars_1_def Pmap_def case_prod_beta fst_conv snd_conv compSS_defs)
+    apply (subst IImsupp_naturals, (rule assms cmin1 cmin2 card_of_Card_order ordLess_ordLeq_trans)+)+
+    apply (unfold image_Un)?
+    apply (rule refl)
+    done
+  subgoal
+    apply (unfold PFVars_2_def Pmap_def case_prod_beta fst_conv snd_conv compSS_defs)
+    apply (subst IImsupp_naturals, (rule assms cmin1 cmin2 card_of_Card_order ordLess_ordLeq_trans)+)+
+    apply (unfold image_Un)?
+    apply (rule refl)
+    done
+  done
+
+lemma Pmap_cong_id:
+  fixes f1::"'tyvar::var \<Rightarrow> 'tyvar" and f2::"'var::var \<Rightarrow> 'var"
+  assumes f_prems: "bij f1" "|supp f1| <o cmin |UNIV::'tyvar set| |UNIV::'var set|" "bij f2" "|supp f2| <o cmin |UNIV::'tyvar set| |UNIV::'var set|"
+  shows "(\<And>a. a \<in> PFVars_1 p \<Longrightarrow> f1 a = a) \<Longrightarrow> (\<And>a. a \<in> PFVars_2 p \<Longrightarrow> f2 a = a) \<Longrightarrow> Pmap f1 f2 p = p"
+  apply (unfold PFVars_1_def PFVars_2_def Pmap_def case_prod_beta)
+  subgoal premises prems
+    apply (subst compSS_cong_ids, (rule f_prems prems cmin1 cmin2 card_of_Card_order ordLess_ordLeq_trans | erule UnI2 UnI1 | rule UnI1)+)+
+    apply assumption
+    apply (unfold prod.collapse)
+    apply (rule refl)
+    done
+  done
+
+lemmas Cinfinite_UNIV = conjI[OF trm_pre.UNIV_cinfinite card_of_Card_order]
+lemmas Cinfinite_card = cmin_Cinfinite[OF Cinfinite_UNIV Cinfinite_UNIV]
+lemmas regularCard_card = cmin_regularCard[OF trm_pre.var_regular trm_pre.var_regular Cinfinite_UNIV Cinfinite_UNIV]
+lemmas Un_bound = regularCard_Un[OF conjunct2[OF Cinfinite_card] conjunct1[OF Cinfinite_card] regularCard_card]
+lemmas UN_bound = regularCard_UNION[OF conjunct2[OF Cinfinite_card] conjunct1[OF Cinfinite_card] regularCard_card]
+
+lemma small_PFVarss:
+  "valid_P p \<Longrightarrow> |PFVars_1 (p::('tyvar::var, 'var::var) P)| <o cmin |UNIV::'tyvar set| |UNIV::'var set|"
+  "valid_P p \<Longrightarrow> |PFVars_2 p| <o cmin |UNIV::'tyvar set| |UNIV::'var set|"
+  subgoal
+    apply (unfold PFVars_1_def case_prod_beta IImsupp_1_trm_def IImsupp_2_trm_def IImsupp_typ_def comp_def valid_P_def)
+    apply (erule conjE)+
+        apply (assumption | rule Un_bound UN_bound ordLeq_ordLess_trans[OF card_of_image] typ.set_bd_UNIV trm.FVars_bd_UNIVs cmin_greater card_of_Card_order)+
+    done
+  (* copied from above *)
+  subgoal
+    apply (unfold PFVars_2_def case_prod_beta IImsupp_1_trm_def IImsupp_2_trm_def IImsupp_typ_def comp_def valid_P_def)
+    apply (erule conjE)+
+        apply (assumption | rule Un_bound UN_bound ordLeq_ordLess_trans[OF card_of_image] typ.set_bd_UNIV trm.FVars_bd_UNIVs cmin_greater card_of_Card_order)+
+    done
+  done
+
+lemma sets_tvsubst_trm_pre:
+  "set2_trm_pre (tvsubst_trm_pre f x) = set2_trm_pre x"
+  "set3_trm_pre (tvsubst_trm_pre f x) = set3_trm_pre x"
+  "set4_trm_pre (tvsubst_trm_pre f x) = set4_trm_pre x"
+  "set5_trm_pre (tvsubst_trm_pre f x) = set5_trm_pre x"
+  "set6_trm_pre (tvsubst_trm_pre f x) = set6_trm_pre x"
+      apply (unfold set2_trm_pre_def set3_trm_pre_def set4_trm_pre_def set5_trm_pre_def set6_trm_pre_def UN_empty
+sum.set_map UN_single UN_singleton UN_empty2 Un_empty_right Un_empty_left prod.set_map tvsubst_trm_pre_def
+  comp_def Abs_trm_pre_inverse[OF UNIV_I]
+  )
+  by (auto split: sum.splits)
+
+lemma map_subst: "tvsubst_trm_pre g (map_trm_pre id f2 f3 f4 f5 f6 x) = map_trm_pre id f2 f3 f4 f5 f6 (tvsubst_trm_pre g x)"
+  apply (unfold tvsubst_trm_pre_def map_trm_pre_def comp_def Abs_trm_pre_inverse[OF UNIV_I] case_sum_map_sum
+    typ.map_id0 case_prod_map_prod
+  )
+  apply (auto split: sum.split)
+  done
+
+lemma FVars_tvsubst:
+  assumes "|SSupp_typ (g::'tv \<Rightarrow> _)| <o cmin |UNIV::'tv::var set| |UNIV::'v::var set|"
+  shows "FVars_typ (tvsubst_typ g x) = \<Union>((FVars_typ \<circ> g) ` FVars_typ x)"
+proof -
+  have a: "|SSupp_typ g| <o |UNIV::'tv set|"
+    apply (rule ordLess_ordLeq_trans)
+      apply (rule assms)
+     apply (rule cmin1)
+     apply (rule card_of_Card_order)+
+    done
+  then show ?thesis
+  proof (binder_induction x avoiding: x "IImsupp_typ g" rule: typ.strong_induct)
+    case Bound
+    then show ?case unfolding IImsupp_typ_def using var_class.Un_bound var_class.UN_bound typ.set_bd_UNIV a
+      by (metis type_copy_set_bd)
+  next
+    case (Forall x1 x2 x3)
+    then show ?case apply auto
+      using IImsupp_typ_def SSupp_typ_def typ.FVars_VVr apply fastforce
+      by (metis singletonD typ.FVars_VVr typ.in_IImsupp)
+  qed (auto simp: lfset.set_map)
+qed
+
+lemma FTVars_subset: "valid_P p \<Longrightarrow> set3_trm_pre y \<inter> PFVars_1 p = {} \<Longrightarrow>
+  (\<And>t pu p. valid_P p \<Longrightarrow> (t, pu) \<in> set5_trm_pre y \<union> set6_trm_pre y \<Longrightarrow> FTVars (pu p) \<subseteq> FTVars t \<union> PFVars_1 p) \<Longrightarrow>
+  FTVars (Uctor y p) \<subseteq> FTVars (trm_ctor (map_trm_pre id id id id fst fst y)) \<union> PFVars_1 p"
+  apply (frule iffD1[OF meta_eq_to_obj_eq[OF valid_P_def]])
+  apply (unfold case_prod_beta)
+  apply (erule conjE)+
+  subgoal premises prems
+    apply (unfold Uctor_def case_prod_beta)
+    apply (rule case_split)
+     apply (subst if_P)
+      apply assumption
+     apply (unfold isVVr_def)[1]
+     apply (erule exE)
+     apply (drule sym)
+    apply (erule subst)
+     apply (unfold asVVr_VVr)
+     apply (rule case_split[of "_ = _"])
+      apply (rule iffD2[OF arg_cong2[OF _ refl, of _ _ "(\<subseteq>)"]])
+       apply (rule arg_cong[of _ _ FTVars])
+       apply assumption
+      apply (rule Un_upper1)
+     apply (rule subsetI)
+     apply (rule UnI2)
+     apply (unfold PFVars_1_def case_prod_beta IImsupp_1_trm_def SSupp_trm_def tvVVr_tvsubst_trm_def tv\<eta>_trm_tvsubst_trm_def VVr_def[symmetric] image_comp[unfolded comp_def])[1]
+     apply (unfold comp_def)[1]
+     apply (rule UnI1)
+     apply (rule UN_I)
+      apply (rule CollectI)
+      apply assumption
+     apply assumption
+    apply (unfold if_not_P)
+    apply (erule thin_rl)
+
+    apply (unfold prod.collapse trm.FVars_ctor sets_tvsubst_trm_pre map_subst)
+    apply (subst trm_pre.set_map, (rule bij_id supp_id_bound)+)+
+    apply (unfold image_id image_comp comp_def prod.collapse)
+    apply (rule Un_mono')+
+    subgoal
+      apply (unfold set1_trm_pre_def tvsubst_trm_pre_def PFVars_1_def UN_empty
+        sum.set_map UN_single UN_singleton UN_empty2 Un_empty_right Un_empty_left prod.set_map tvsubst_trm_pre_def
+        comp_def Abs_trm_pre_inverse[OF UNIV_I] IImsupp_1_trm_def IImsupp_typ_def SSupp_typ_def fst_conv snd_conv
+        tvVVr_tvsubst_typ_def tv\<eta>_typ_tvsubst_typ_def TyVar_def[symmetric] map_trm_pre_def typ.map_id0
+        SSupp_trm_def tvVVr_tvsubst_trm_def tv\<eta>_trm_tvsubst_trm_def VVr_def[symmetric] typ.set_map
+      )
+      using prems(4,5) apply (auto split: sum.splits simp: FVars_tvsubst)
+        apply (metis singletonD typ.set(1))+
+      done
+    apply (rule iffD2[OF arg_cong2[OF refl, of _ _ "(\<subseteq>)"]])
+      apply (rule Diff_Un_disjunct)
+      apply (rule prems)
+    apply (unfold sets_tvsubst_trm_pre)
+     apply (rule Diff_mono[OF _ subset_refl])
+     apply (unfold UN_extend_simps(2))
+      (* REPEAT_DETERM *)
+     apply (rule subset_If)
+      apply (unfold UN_empty')[1]
+      apply (rule empty_subsetI)
+     apply (rule UN_mono[OF subset_refl])
+     apply (rule prems)
+      apply (rule prems)
+     apply (unfold prod.collapse)
+     apply (erule UnI2 UnI1)
+    (* repeated *)
+     apply (rule subset_If)
+      apply (unfold UN_empty')[1]
+      apply (rule empty_subsetI)
+     apply (rule UN_mono[OF subset_refl])
+     apply (rule prems)
+      apply (rule prems)
+     apply (unfold prod.collapse)
+     apply (erule UnI2 UnI1)
+    (* END REPEAT_DETERM *)
+    done
+  done
+
+lemma FVars_subset: "valid_P p \<Longrightarrow> set4_trm_pre y \<inter> PFVars_2 p = {} \<Longrightarrow>
+  (\<And>t pu p. valid_P p \<Longrightarrow> (t, pu) \<in> set5_trm_pre y \<union> set6_trm_pre y \<Longrightarrow> FVars (pu p) \<subseteq> FVars t \<union> PFVars_2 p) \<Longrightarrow>
+  FVars (Uctor y p) \<subseteq> FVars (trm_ctor (map_trm_pre id id id id fst fst y)) \<union> PFVars_2 p"
+  apply (frule iffD1[OF meta_eq_to_obj_eq[OF valid_P_def]])
+  apply (unfold case_prod_beta)
+  apply (erule conjE)+
+  subgoal premises prems
+    apply (unfold Uctor_def case_prod_beta)
+    apply (rule case_split)
+     apply (subst if_P)
+      apply assumption
+     apply (unfold isVVr_def)[1]
+     apply (erule exE)
+     apply (drule sym)
+    apply (erule subst)
+     apply (unfold asVVr_VVr)
+     apply (rule case_split[of "_ = _"])
+      apply (rule iffD2[OF arg_cong2[OF _ refl, of _ _ "(\<subseteq>)"]])
+       apply (rule arg_cong[of _ _ FVars])
+       apply assumption
+      apply (rule Un_upper1)
+     apply (rule subsetI)
+     apply (rule UnI2)
+     apply (unfold PFVars_2_def case_prod_beta IImsupp_2_trm_def SSupp_trm_def tvVVr_tvsubst_trm_def tv\<eta>_trm_tvsubst_trm_def VVr_def[symmetric] image_comp[unfolded comp_def])[1]
+    apply (rule UnI2)
+     apply (rule UN_I)
+      apply (rule CollectI)
+      apply assumption
+     apply (unfold comp_def)[1]
+     apply assumption
+    apply (unfold if_not_P)
+    apply (erule thin_rl)
+
+    apply (unfold trm.FVars_ctor prod.collapse sets_tvsubst_trm_pre map_subst)
+    apply (subst trm_pre.set_map, (rule bij_id supp_id_bound)+)+
+    apply (unfold image_id image_comp comp_def prod.collapse sets_tvsubst_trm_pre)
+    apply (rule Un_mono')+
+      apply (rule Un_upper1)
+    apply (rule iffD2[OF arg_cong2[OF refl, of _ _ "(\<subseteq>)"]])
+      apply (rule Diff_Un_disjunct)
+      apply (rule prems)
+     apply (rule Diff_mono[OF _ subset_refl])
+     apply (unfold UN_extend_simps(2))
+      (* REPEAT_DETERM *)
+     apply (rule subset_If)
+      apply (unfold UN_empty')[1]
+      apply (rule empty_subsetI)
+     apply (rule UN_mono[OF subset_refl])
+     apply (rule prems)
+      apply (rule prems)
+     apply (unfold prod.collapse)
+     apply (erule UnI2 UnI1)
+    (* repeated *)
+     apply (rule subset_If)
+      apply (unfold UN_empty')[1]
+      apply (rule empty_subsetI)
+     apply (rule UN_mono[OF subset_refl])
+     apply (rule prems)
+      apply (rule prems)
+     apply (unfold prod.collapse)
+     apply (erule UnI2 UnI1)
+    (* END REPEAT_DETERM *)
+    done
+  done
+
+lemma permute_Uctor:
+  fixes f1::"'tv::var \<Rightarrow> 'tv" and f2::"'v::var \<Rightarrow> 'v"
+  shows "valid_P p \<Longrightarrow> bij f1 \<Longrightarrow> |supp f1| <o cmin |UNIV::'tv set| |UNIV::'v set| \<Longrightarrow> bij f2 \<Longrightarrow> |supp f2| <o cmin |UNIV::'tv set| |UNIV::'v set|
+  \<Longrightarrow> permute_trm f1 f2 (Uctor y p) = Uctor (map_trm_pre f1 f2 f1 f2
+    (\<lambda>(t, pu). (permute_trm f1 f2 t, \<lambda>p. if valid_P p then permute_trm f1 f2 (pu (Pmap (inv f1) (inv f2) p)) else undefined))
+    (\<lambda>(t, pu). (permute_trm f1 f2 t, \<lambda>p. if valid_P p then permute_trm f1 f2 (pu (Pmap (inv f1) (inv f2) p)) else undefined))
+  y) (Pmap f1 f2 p)"
+  apply (frule iffD1[OF meta_eq_to_obj_eq[OF valid_P_def]])
+  apply (subst (asm) case_prod_beta)
+  apply (erule conjE)+
+  apply (unfold Uctor_def)
+  apply (subst trm_pre.map_comp, (assumption | rule supp_id_bound bij_id ordLess_ordLeq_trans cmin1 cmin2 card_of_Card_order)+)+
+  apply (unfold id_o_commute[of f1] id_o_commute[of f2] fst_o_f comp_assoc comp_def[of snd] snd_conv case_prod_beta prod.collapse)
+  apply (subst trm_pre.map_comp[symmetric], (assumption | rule supp_id_bound bij_id ordLess_ordLeq_trans cmin1 cmin2 card_of_Card_order)+)+
+  apply (subst trm.permute_ctor[symmetric] isVVr_permute, (assumption | rule ordLess_ordLeq_trans cmin1 cmin2 card_of_Card_order)+)+
+
+  apply (rule case_split)
+   apply (subst if_P)
+    apply assumption
+   apply (unfold if_P if_not_P)
+   apply (unfold isVVr_def)[1]
+   apply (erule exE)
+   apply (erule subst[OF sym])
+   apply (subst permute_VVr)
+       apply (assumption | rule ordLess_ordLeq_trans cmin1 cmin2 card_of_Card_order)+
+   apply (unfold Pmap_def case_prod_beta fst_conv snd_conv asVVr_VVr compSS_trm_def comp_def)[1]
+   apply (subst inv_simp1)
+    apply assumption
+   apply (rule refl)
+
+  apply (rule trans)
+   apply (rule trm.permute_ctor)
+      apply (assumption | rule ordLess_ordLeq_trans cmin1 cmin2 card_of_Card_order)+
+  apply (unfold map_subst)
+
+  apply (subst trm_pre.map_comp, (assumption | rule supp_id_bound bij_id ordLess_ordLeq_trans cmin1 cmin2 card_of_Card_order)+)+
+  apply (unfold id_o o_id)
+  apply (unfold comp_def)
+  apply (subst if_P inv_o_simp1 trans[OF comp_apply[symmetric] Pmap_comp0[THEN fun_cong]], (rule valid_Pmap bij_imp_bij_inv supp_inv_bound | assumption)+)+
+  apply (unfold trans[OF Pmap_id0[THEN fun_cong] id_apply])
+  apply (unfold Pmap_def case_prod_beta snd_conv compSS_typ_def)
+  apply (rule arg_cong[of _ _ trm_ctor])
+
+  apply (unfold tvsubst_trm_pre_def map_trm_pre_def comp_def typ.map_id0 Abs_trm_pre_inverse[OF UNIV_I])
+  apply (frule ordLess_ordLeq_trans)
+   apply (rule cmin1 card_of_Card_order)+
+  apply (rotate_tac -3)
+  apply (unfold typ.vvsubst_permute)
+  apply (frule ordLess_ordLeq_trans)
+   apply (rule cmin1 card_of_Card_order)+
+  apply (auto split: sum.splits simp: Abs_trm_pre_inject trans[OF comp_apply[symmetric] typ.tvsubst_permutes[THEN fun_cong]] comp_def)
+  done
+
+ML \<open>
+val nvars: int = 2
+val parameters = {
+  P = @{typ "('tv::var, 'v::var) P"},
+  Pmap = @{term "Pmap :: _ \<Rightarrow> _ \<Rightarrow> _ \<Rightarrow> ('tv::var, 'v::var) P"},
+  PFVarss = [
+    @{term "PFVars_1 :: ('tv::var, 'v::var) P \<Rightarrow> _"},
+    @{term "PFVars_2 :: ('tv::var, 'v::var) P \<Rightarrow> _"}
+  ],
+  avoiding_sets = [@{term "{} :: 'tv::var set"}, @{term "{} :: 'v::var set"}],
+  min_bound = true,
+  validity = SOME {
+    pred = @{term "valid_P :: ('tv::var, 'v::var) P \<Rightarrow> _"},
+    valid_Pmap = fn ctxt => HEADGOAL (resolve_tac ctxt @{thms valid_Pmap} THEN_ALL_NEW assume_tac ctxt)
+  },
+  axioms = {
+    Pmap_id0 = fn ctxt => EVERY1 [
+      resolve_tac ctxt [trans],
+      resolve_tac ctxt @{thms fun_cong[OF Pmap_id0]},
+      resolve_tac ctxt @{thms id_apply}
+    ],
+    Pmap_comp0 = fn ctxt => resolve_tac ctxt @{thms fun_cong[OF Pmap_comp0[symmetric]]} 1 THEN REPEAT_DETERM (assume_tac ctxt 1),
+    Pmap_cong_id = fn ctxt => resolve_tac ctxt @{thms Pmap_cong_id} 1 THEN REPEAT_DETERM (assume_tac ctxt 1 ORELSE Goal.assume_rule_tac ctxt 1),
+    PFVars_Pmaps = replicate nvars (fn ctxt => resolve_tac ctxt @{thms PFVars_Pmaps} 1 THEN REPEAT_DETERM (assume_tac ctxt 1)),
+    small_PFVarss = replicate nvars (fn ctxt => resolve_tac ctxt @{thms small_PFVarss} 1 THEN assume_tac ctxt 1),
+    small_avoiding_sets = replicate nvars (fn ctxt => HEADGOAL (resolve_tac ctxt @{thms cmin_greater}
+      THEN_ALL_NEW resolve_tac ctxt @{thms card_of_Card_order emp_bound}))
+  }
+} : (Proof.context -> tactic) MRBNF_Recursor.parameter;
+\<close>
+
+ML \<open>
+val fp_res = the (MRBNF_FP_Def_Sugar.fp_result_of @{context} "POPLmark_2B.trm")
+val quot = hd (#quotient_fps fp_res);
+val vars = map TVar (rev (Term.add_tvarsT (#T quot) []));
+\<close>
+
+ML \<open>
+val model = MRBNF_Recursor.mk_quotient_model quot (vars ~~ [@{typ "'tv::var"}, @{typ "'v::var"}]) {
+  binding = @{binding "tvsubst"},
+  Uctor = @{term "Uctor :: _ \<Rightarrow> ('tv::var, 'v::var) P \<Rightarrow> _"},
+  validity = NONE,
+  axioms = {
+    FVars_subsets = [
+      fn ctxt => EVERY1 [
+        K (Local_Defs.unfold0_tac ctxt @{thms Un_empty_right}),
+        resolve_tac ctxt @{thms FTVars_subset},
+        REPEAT_DETERM o assume_tac ctxt,
+        Goal.assume_rule_tac ctxt
+      ],
+      fn ctxt => EVERY1 [
+        K (Local_Defs.unfold0_tac ctxt @{thms Un_empty_right}),
+        resolve_tac ctxt @{thms FVars_subset},
+        REPEAT_DETERM o assume_tac ctxt,
+        Goal.assume_rule_tac ctxt
+      ]
+    ],
+    permute_Uctor = fn ctxt => HEADGOAL (resolve_tac ctxt @{thms permute_Uctor} THEN_ALL_NEW assume_tac ctxt)
+  }
+}
+\<close>
+
+local_setup \<open>fn lthy =>
+let
+  val qualify = I
+  val (ress, lthy) = MRBNF_Recursor.create_binding_recursor qualify fp_res parameters [model] lthy
+  val notes =
+    [ ("rec_Uctor", map (Local_Defs.unfold0 lthy @{thms Un_empty_right} o #rec_Uctor) ress)
+    ] |> (map (fn (thmN, thms) =>
+      ((Binding.qualify true "trm" (Binding.name thmN), []), [(thms, [])])
+    ));
+  val (_, lthy) = Local_Theory.notes notes lthy
+  val _ = @{print} ress
+in lthy end
+\<close>
+print_theorems
+
+definition tvsubst :: "('v \<Rightarrow> ('tv::var, 'v::var) trm) \<Rightarrow> ('tv \<Rightarrow> 'tv typ) \<Rightarrow> ('tv, 'v) trm \<Rightarrow> ('tv, 'v) trm" where
+  "tvsubst f1 f2 t \<equiv> ff0_tvsubst t (f1, f2)"
+
+type_synonym ('tv, 'v) U1_pre = "('tv, 'v, 'tv, 'v, ('tv, 'v) trm, ('tv, 'v) trm) trm_pre"
+
+lemmas eta_natural' = fun_cong[OF eta_natural, unfolded comp_def]
+lemma eta_set_empties:
+  fixes a::"'v::var"
+  shows
+    "set1_trm_pre (\<eta> a :: ('tv::var, 'v) U1_pre) = {}"
+    "set3_trm_pre (\<eta> a :: ('tv::var, 'v) U1_pre) = {}"
+    "set4_trm_pre (\<eta> a :: ('tv::var, 'v) U1_pre) = {}"
+    "set5_trm_pre (\<eta> a :: ('tv::var, 'v) U1_pre) = {}"
+    "set6_trm_pre (\<eta> a :: ('tv::var, 'v) U1_pre) = {}"
+      apply -
+  subgoal
+    apply (rule set_eqI)
+    apply (unfold empty_iff)
+    apply (rule iffI)
+     apply (rule exE[OF MRBNF_FP.exists_fresh, of "set1_trm_pre (\<eta> a)"])
+      apply (rule trm_pre.set_bd_UNIV)
+     apply (drule iffD1[OF arg_cong2[OF refl, of _ _ "(\<in>)"], rotated])
+      apply (rule arg_cong[of _ _ set1_trm_pre])
+      prefer 2
+      apply (subst (asm) trm_pre.set_map)
+            prefer 7
+            apply (erule swap_fresh)
+            apply assumption
+           apply (rule supp_id_bound bij_id supp_swap_bound bij_swap infinite_UNIV)+
+     apply (rule sym)
+     apply (rule trans)
+      apply (rule fun_cong[OF eta_natural, unfolded comp_def])
+           apply (rule supp_id_bound bij_id supp_swap_bound bij_swap infinite_UNIV)+
+     apply (unfold id_def)
+     apply (rule refl)
+    apply (erule FalseE)
+    done
+  subgoal
+    apply (rule set_eqI)
+    apply (unfold empty_iff)
+    apply (rule iffI)
+     apply (rule exE[OF MRBNF_FP.exists_fresh, of "set3_trm_pre (\<eta> a)"])
+      apply (rule trm_pre.set_bd_UNIV)
+     apply (drule iffD1[OF arg_cong2[OF refl, of _ _ "(\<in>)"], rotated])
+      apply (rule arg_cong[of _ _ set3_trm_pre])
+      prefer 2
+      apply (subst (asm) trm_pre.set_map)
+            prefer 7
+            apply (erule swap_fresh)
+            apply assumption
+           apply (rule supp_id_bound bij_id supp_swap_bound bij_swap infinite_UNIV)+
+     apply (rule sym)
+     apply (rule trans)
+      apply (rule fun_cong[OF eta_natural, unfolded comp_def])
+           apply (rule supp_id_bound bij_id supp_swap_bound bij_swap infinite_UNIV)+
+     apply (unfold id_def)
+     apply (rule refl)
+    apply (erule FalseE)
+    done
+  subgoal
+    apply (rule set_eqI)
+    apply (unfold empty_iff)
+    apply (rule iffI)
+     apply (rule exE[OF MRBNF_FP.exists_fresh, of "set4_trm_pre (\<eta> a)"])
+      apply (rule trm_pre.set_bd_UNIV)
+     apply (drule iffD1[OF arg_cong2[OF refl, of _ _ "(\<in>)"], rotated])
+      apply (rule arg_cong[of _ _ set4_trm_pre])
+      prefer 2
+      apply (subst (asm) trm_pre.set_map)
+            prefer 7
+            apply (erule swap_fresh)
+            apply assumption
+           apply (rule supp_id_bound bij_id supp_swap_bound bij_swap infinite_UNIV)+
+     apply (rule sym)
+     apply (rule trans)
+      apply (rule eta_natural')
+           apply (rule supp_id_bound bij_id supp_swap_bound bij_swap infinite_UNIV)+
+     apply (unfold id_def)
+     apply (rule refl)
+    apply (erule FalseE)
+    done
+  subgoal
+    apply (rule set_eqI)
+    apply (unfold empty_iff)
+    apply (rule iffI)
+     apply (drule image_const)
+     apply (drule iffD1[OF all_cong1, rotated])
+      apply (rule sym)
+      apply (rule arg_cong2[OF refl, of _ _ "(\<in>)"])
+      apply (rule trm_pre.set_map)
+           apply (rule supp_id_bound bij_id)+
+     apply (subst (asm) eta_natural')
+         apply (rule supp_id_bound bij_id)+
+     apply (unfold id_def)
+     apply (drule forall_in_eq_UNIV)
+     apply (drule trans[symmetric])
+      apply (rule conjunct1[OF card_order_on_Card_order, OF trm_pre.bd_card_order])
+     apply (drule card_of_ordIso_subst)
+     apply (drule ordIso_symmetric)
+     apply (drule ordIso_transitive)
+      apply (rule ordIso_symmetric)
+      apply (rule iffD1[OF Card_order_iff_ordIso_card_of])
+      apply (rule conjunct2[OF card_order_on_Card_order, OF trm_pre.bd_card_order])
+     apply (erule ordIso_ordLess_False)
+     apply (rule trm_pre.set_bd)
+    apply (erule FalseE)
+    done
+  subgoal
+    apply (rule set_eqI)
+    apply (unfold empty_iff)
+    apply (rule iffI)
+     apply (drule image_const)
+     apply (drule iffD1[OF all_cong1, rotated])
+      apply (rule sym)
+      apply (rule arg_cong2[OF refl, of _ _ "(\<in>)"])
+      apply (rule trm_pre.set_map)
+           apply (rule supp_id_bound bij_id)+
+     apply (subst (asm) eta_natural')
+         apply (rule supp_id_bound bij_id)+
+     apply (unfold id_def)
+     apply (drule forall_in_eq_UNIV)
+     apply (drule trans[symmetric])
+      apply (rule conjunct1[OF card_order_on_Card_order, OF trm_pre.bd_card_order])
+     apply (drule card_of_ordIso_subst)
+     apply (drule ordIso_symmetric)
+     apply (drule ordIso_transitive)
+      apply (rule ordIso_symmetric)
+      apply (rule iffD1[OF Card_order_iff_ordIso_card_of])
+      apply (rule conjunct2[OF card_order_on_Card_order, OF trm_pre.bd_card_order])
+     apply (erule ordIso_ordLess_False)
+     apply (rule trm_pre.set_bd)
+    apply (erule FalseE)
+    done
+  done
+
+lemma tvsubst_VVr:
+  assumes
+    "|SSupp_trm f1| <o cmin |UNIV::'tv set| |UNIV::'v set|"
+    "|SSupp_typ f2| <o cmin |UNIV::'tv set| |UNIV::'v set|"
+  shows "tvsubst f1 f2 (VVr a :: ('tv::var, 'v::var) trm) = f1 a"
+  apply (unfold tvsubst_def VVr_def comp_def)
+  apply (rule trans)
+   apply (rule trm.rec_Uctor)
+      apply (unfold valid_P_def prod.case)
+      apply (rule conjI assms)+
+     apply (unfold eta_set_empties noclash_trm_def Uctor_def Un_empty prod.case)
+     apply (rule Int_empty_left conjI)+
+  apply (subst trm_pre.map_comp, (rule supp_id_bound bij_id)+)+
+  apply (unfold id_o o_id comp_def[of fst] fst_conv id_def[symmetric] trm_pre.map_id)
+  apply (rule trans)
+   apply (rule if_P)
+   apply (unfold isVVr_def VVr_def comp_def )
+   apply (rule exI)
+   apply (rule refl)
+  apply (unfold meta_eq_to_obj_eq[OF VVr_def, THEN fun_cong, unfolded comp_def, symmetric] asVVr_VVr)
+  apply (rule refl)
+  done
+
+lemma tvsubst_not_is_VVr:
+  fixes x::"('tv::var, 'v::var) U1_pre"
+  assumes f_prems: "|SSupp_trm f1| <o cmin |UNIV::'tv set| |UNIV::'v set|" "|SSupp_typ f2| <o cmin |UNIV::'tv set| |UNIV::'v set|"
+    and empty_prems: "set3_trm_pre x \<inter> (IImsupp_1_trm f1 \<union> IImsupp_typ f2) = {}" "set4_trm_pre x \<inter> IImsupp_2_trm f1 = {}"
+    and noclash: "noclash_trm x"
+    and VVr_prems: "\<not>isVVr (trm_ctor x)"
+  shows
+    "tvsubst f1 f2 (trm_ctor x) = trm_ctor (tvsubst_trm_pre f2 (map_trm_pre id id id id (tvsubst f1 f2) (tvsubst f1 f2) x))"
+  apply (unfold tvsubst_def)
+  apply (subgoal_tac "valid_P (f1, f2)")
+   prefer 2
+   apply (unfold valid_P_def prod.case)[1]
+   apply (rule conjI f_prems)+
+  apply (rule trans)
+   apply (rule trm.rec_Uctor)
+      apply assumption
+     apply (unfold PFVars_1_def PFVars_2_def prod.case)
+     apply (rule empty_prems noclash)+
+  apply (unfold Uctor_def prod.case)
+  apply (subst trm_pre.map_comp, (rule supp_id_bound bij_id)+)+
+  apply (unfold id_o o_id comp_def[of fst] fst_conv id_def[symmetric] trm_pre.map_id)
+  apply (subst if_not_P, rule VVr_prems)+
+  apply (unfold comp_def snd_conv if_P)
+  apply (rule refl)
+  done
+
+lemma tvsubst_simps[simp]:
+  fixes f1::"'v \<Rightarrow> ('tv::var, 'v::var) trm" and f2::"'tv \<Rightarrow> 'tv typ"
+  assumes f_prems: "|SSupp_trm f1| <o cmin |UNIV::'tv set| |UNIV::'v set|" "|SSupp_typ f2| <o cmin |UNIV::'tv set| |UNIV::'v set|"
+  shows
+    "tvsubst f1 f2 (Var x) = f1 x"
+    "x \<notin> IImsupp_2_trm f1 \<Longrightarrow> tvsubst f1 f2 (Abs x T t) = Abs x (tvsubst_typ f2 T) (tvsubst f1 f2 t)"
+    "tvsubst f1 f2 (App t1 t2) = App (tvsubst f1 f2 t1) (tvsubst f1 f2 t2)"
+    "X \<notin> IImsupp_1_trm f1 \<Longrightarrow> X \<notin> IImsupp_typ f2 \<Longrightarrow> X \<notin> FVars_typ T \<Longrightarrow> tvsubst f1 f2 (TAbs X T t) = TAbs X (tvsubst_typ f2 T) (tvsubst f1 f2 t)"
+    "tvsubst f1 f2 (TApp t T) = TApp (tvsubst f1 f2 t) (tvsubst_typ f2 T)"
+  subgoal
+    apply (unfold Var_def VVr_def[unfolded comp_def, symmetric, THEN meta_eq_to_obj_eq, THEN fun_cong])
+    apply (rule tvsubst_VVr)
+     apply (rule assms)+
+    done
+  subgoal
+  apply (unfold Abs_def)
+  apply (rule trans[OF tvsubst_not_is_VVr])
+        apply (rule assms)+
+      apply (unfold set3_trm_pre_def set4_trm_pre_def sum.set_map UN_empty UN_empty2 Un_empty_left comp_def
+        Abs_trm_pre_inverse[OF UNIV_I] sum_set_simps UN_single prod.set_map prod_set_simps Un_empty_right
+        noclash_trm_def set1_trm_pre_def set6_trm_pre_def set2_trm_pre_def isVVr_def VVr_def
+        Abs_trm_pre_inject[OF UNIV_I UNIV_I] trm.TT_inject0 set5_trm_pre_def map_trm_pre_def
+        map_prod_simp map_sum.simps
+      )[4]
+       apply (auto split: sum.splits simp: tvsubst_trm_pre_def trm.TT_inject0 map_trm_pre_def Abs_trm_pre_inverse typ.map_id)
+    done
+  subgoal
+  apply (unfold App_def)
+  apply (rule trans[OF tvsubst_not_is_VVr])
+        apply (rule assms)+
+      apply (unfold set3_trm_pre_def set4_trm_pre_def sum.set_map UN_empty UN_empty2 Un_empty_left comp_def
+        Abs_trm_pre_inverse[OF UNIV_I] sum_set_simps UN_single prod.set_map prod_set_simps Un_empty_right
+        noclash_trm_def set1_trm_pre_def set6_trm_pre_def set2_trm_pre_def isVVr_def VVr_def
+        Abs_trm_pre_inject[OF UNIV_I UNIV_I] trm.TT_inject0 set5_trm_pre_def map_trm_pre_def
+        map_prod_simp map_sum.simps
+      )[4]
+       apply (auto split: sum.splits simp: tvsubst_trm_pre_def trm.TT_inject0 map_trm_pre_def Abs_trm_pre_inverse typ.map_id)
+    done
+  subgoal
+  apply (unfold TAbs_def)
+  apply (rule trans[OF tvsubst_not_is_VVr])
+        apply (rule assms)+
+      apply (unfold set3_trm_pre_def set4_trm_pre_def sum.set_map UN_empty UN_empty2 Un_empty_left comp_def
+        Abs_trm_pre_inverse[OF UNIV_I] sum_set_simps UN_single prod.set_map prod_set_simps Un_empty_right
+        noclash_trm_def set1_trm_pre_def set6_trm_pre_def set2_trm_pre_def isVVr_def VVr_def
+        Abs_trm_pre_inject[OF UNIV_I UNIV_I] trm.TT_inject0 set5_trm_pre_def map_trm_pre_def
+        map_prod_simp map_sum.simps
+      )[4]
+       apply (auto split: sum.splits simp: tvsubst_trm_pre_def trm.TT_inject0 map_trm_pre_def Abs_trm_pre_inverse typ.map_id)
+    done
+  subgoal
+  apply (unfold TApp_def)
+  apply (rule trans[OF tvsubst_not_is_VVr])
+        apply (rule assms)+
+      apply (unfold set3_trm_pre_def set4_trm_pre_def sum.set_map UN_empty UN_empty2 Un_empty_left comp_def
+        Abs_trm_pre_inverse[OF UNIV_I] sum_set_simps UN_single prod.set_map prod_set_simps Un_empty_right
+        noclash_trm_def set1_trm_pre_def set6_trm_pre_def set2_trm_pre_def isVVr_def VVr_def
+        Abs_trm_pre_inject[OF UNIV_I UNIV_I] trm.TT_inject0 set5_trm_pre_def map_trm_pre_def
+        map_prod_simp map_sum.simps
+      )[4]
+       apply (auto split: sum.splits simp: tvsubst_trm_pre_def trm.TT_inject0 map_trm_pre_def Abs_trm_pre_inverse typ.map_id)
+    done
+  done
+
+(* END OF MANUAL tvsubst construction *)
 
 inductive "value" where
   "value (Abs x T t)"
